# Cartesian Plane
Noted R²
Two axis, X & Y
A = (2, 3) (x, y)
Origin as (0, 0)
Sadly same symbol as open interval
Sometimes use [] with numbers stacked

X Axis = set of all points where y coordinate is 0
Y Axis = set of all points where x coordinate is 0

4 Quadrants
1st quadrant = (x,y) ∈ R² : x > 0, y > 0
2nd quadrant = (x,y) ∈ R² : x < 0, y > 0
3rd quadrant = (x,y) ∈ R² : x < 0, y < 0
4th quadrant = (x,y) ∈ R² : x > 0, y < 0

Measure height and weight in 3 people (cm & kg)
A = 177cm, 88.3kg avg US male
B = 164cm, 74.7kg avg US female
C = etc.

# Distance in the Plane
Distance Formula - Pythagrean Theorem
z² = x² + y²

Dist(A, C) = sqrt((C-A)² + (D-B)²)

Nearest Neighbor
Next point with the shortest distance, may have 2nd neighbor and so on

Clustering
Group of points with distances shorter than distance to points in other cluster
If A and B are in cluster 1
and C is in cluster 2
and D is in cluster 3
then distance between A & B << distance between A & C and << distance between A & D

# Point-Slope Formula
y-y₀ = M(x-x₀)
Slope intercept formula = y = Mx + b

Slope of a line segment
Slope (M) of 	⟶ = (y-y₀) / (x-x₀) or rise / run
			 	AB

A = (1,2)
B = (3,3) 

M = (3-2) / (3-1) = 1/2
run 1 unit rise 0.5 or 1/2 units
This is Positive slope example

C = (-1, 1)
D = (0, 0)
(0-1) / (0--1) = -1/1 = -1
Negative slope

A = (2, 1)
B = (3, 2)
Slope = (2-1)/(3-2) = 1
but continue line infinitely in both directions
All points on line must have same slope
Any point = y-1 = 1(x-2)
(1 = slope)
(3, 2) = 2-1 = 1(3-2) = 1 = 1 so true

Point slope Formula = if line l has slope M and if (x₀, y₀) is any point on line then l has equation y-y₀ = M(x-x₀)

For line l
has point (2,1)
slope = 1
Know point slope formula is y-1 = 1(x-2)
Derive slope intercept formula from this (where X=0) the y intercept
(0,b)
b-1 = 1(0-2)
b-1 = -2
b = -1

y = mx + b

if line l has slope M and l hits Y axis at (0, b) then y = mx + b is line equation
M = tells angle of line
b = where to anchor on y axis

l = (1, 1) & (3, 0)
M = (1-0) / (1-3) = -1/2
y - 1 = -1/2(x-1)

y = -1/2 (0) + b
	